FreeST/StandardLib/SecureChannel.fst
@@ -1,11 +1,15 @@
+--TODO:
+-- Confirm that new nounces are being created per message as expected and that both sides are maintaingin the same state (rng).
+-- Add Poly1305 tag generation and verification.
+
 module SecureChannel where
 
 import SecureUtils
 import DiffieHellman
-import ChaCha20
+import ChaCha20Poly1305
 import RSA
 
-type EstablishSecureChannelA = DHProtocol ; Newchacha20Exchange
+type EstablishSecureChannelA = DHProtocol ; NewChaChaPolyExchange
 type EstablishSecureChannelB = dualof EstablishSecureChannelA
 
 
@@ -13,31 +17,31 @@ type EstablishSecureChannelB = dualof EstablishSecureChannelA
 
 establishSecureChannelA : forall a . EstablishSecureChannelA ; a -> (a, SecureChannelState)
 establishSecureChannelA c =
-    let (c, key) = dhA @(Newchacha20Exchange ; a) c in
-    let (nextCrypt, c) = newChaCha20A @a c in
+    let (c, key) = dhA @(NewChaChaPolyExchange ; a) c in
+    let (nextCrypt, c) = newChaChaPolyA @a c in
     (c, SecureChannelState (key, nextCrypt))
 
 establishSecureChannelB : forall a . EstablishSecureChannelB ; a -> (a, SecureChannelState)
 establishSecureChannelB c =
-    let (c, key) = dhB @(dualof Newchacha20Exchange ; a) c in
-    let (nextCrypt, c) = newChaCha20B @a c in
+    let (c, key) = dhB @(dualof NewChaChaPolyExchange ; a) c in
+    let (nextCrypt, c) = newChaChaPolyB @a c in
     (c, SecureChannelState (key, nextCrypt))
 
 
 --Signed Cypher Suit : DiffieHellman + RSA + chacha20
 
 establishSecureAuthenticatedChannelA : forall a . String -> String -> EstablishSecureChannelA ; a -> (a, SecureChannelState)
-establishSecureAuthenticatedChannelA piKeyString puKeyString c =
-    let piKey = getKeyFromFile piKeyString in
-    let puKey = getKeyFromFile puKeyString in
-    let (c, key) = signedDHA @(Newchacha20Exchange ; a) piKey puKey c in
-    let (nextCrypt, c) = newChaCha20A @a c in
+establishSecureAuthenticatedChannelA piKeyPath puKeyPath c =
+    let piKey = getKeyFromFile piKeyPath in
+    let puKey = getKeyFromFile puKeyPath in
+    let (c, key) = signedDHA @(NewChaChaPolyExchange ; a) piKey puKey c in
+    let (nextCrypt, c) = newChaChaPolyA @a c in
     (c, SecureChannelState (key, nextCrypt))
 
 establishSecureAuthenticatedChannelB : forall a . String -> String -> EstablishSecureChannelB ; a -> (a, SecureChannelState)
-establishSecureAuthenticatedChannelB piKeyString puKeyString c =
-    let piKey = getKeyFromFile piKeyString in
-    let puKey = getKeyFromFile puKeyString in
-    let (c, key) = signedDHB @(dualof Newchacha20Exchange ; a) piKey puKey c in
-    let (nextCrypt, c) = newChaCha20B @a c in
+establishSecureAuthenticatedChannelB piKeyPath puKeyPath c =
+    let piKey = getKeyFromFile piKeyPath in
+    let puKey = getKeyFromFile puKeyPath in
+    let (c, key) = signedDHB @(dualof NewChaChaPolyExchange ; a) piKey puKey c in
+    let (nextCrypt, c) = newChaChaPolyB @a c in
     (c, SecureChannelState (key, nextCrypt))
